Sprinkle around some cheats to get things to build

compiler/backend/passes/proofs/env_to_stateProofScript.sml
@@ -52,8 +52,9 @@ Definition cexp_wf_def[simp]:
     (EVERY I (MAP (λ(_,x). cexp_wf x) fs) ∧ cexp_wf x ∧
      ALL_DISTINCT (MAP (λx. explode (FST x)) fs) ∧
      EVERY (λ(_,x). ∃n m. x = Lam n m ∨ x = Delay m) fs) ∧
-  cexp_wf (Case x v rs) =
-    (EVERY I (MAP (λ(_,_,x). cexp_wf x) rs) ∧ cexp_wf x ∧
+  cexp_wf (Case v rs x) =
+    (EVERY I (MAP (λ(_,_,x). cexp_wf x) rs) ∧
+     OPTION_ALL (λ(_,x). cexp_wf x) x ∧
      DISJOINT (set (MAP (explode o FST) rs)) monad_cns ∧
      ALL_DISTINCT (MAP FST rs) ∧
      ~MEM v (FLAT (MAP (FST o SND) rs))) ∧
@@ -95,30 +96,51 @@ QED
 Theorem unthunk_lets_for:
   ∀xs v h1 h2.
     unthunk h1 h2 ⇒
-    unthunk (state_caseProof$lets_for v s xs h1)
-            (state_caseProof$lets_for v s xs h2)
+    unthunk (state_caseProof$lets_for l v s xs h1)
+            (state_caseProof$lets_for l v s xs h2)
 Proof
   Induct \\ fs [state_caseProofTheory.lets_for_def]
   \\ PairCases \\ fs [state_caseProofTheory.lets_for_def] \\ rw []
   \\ irule_at Any state_unthunkProofTheory.compile_rel_Let \\ fs []
-  \\ irule_at Any state_unthunkProofTheory.compile_rel_App \\ fs []
+  \\ irule_at Any state_unthunkProofTheory.compile_rel_Let \\ fs []
+  \\ irule_at Any state_unthunkProofTheory.compile_rel_If \\ fs []
+  \\ rpt (irule_at Any state_unthunkProofTheory.compile_rel_App \\ fs [])
   \\ irule_at Any state_unthunkProofTheory.compile_rel_Var \\ fs []
 QED
 
+Theorem unthnk_Disj:
+  ∀x s. unthunk (state_caseProof$Disj s x) (state_caseProof$Disj s x)
+Proof
+  Induct
+  \\ fs [state_caseProofTheory.Disj_def,FORALL_PROD] \\ rw []
+  \\ rpt (irule_at Any state_unthunkProofTheory.compile_rel_App \\ fs [])
+  \\ rpt (irule_at Any state_unthunkProofTheory.compile_rel_If \\ fs [])
+  \\ rpt (irule_at Any state_unthunkProofTheory.compile_rel_App \\ fs [])
+  \\ rpt (irule_at Any state_unthunkProofTheory.compile_rel_Var \\ fs [])
+QED
+
 Theorem unthunk_rows_of:
-  ∀xs ys s.
+  ∀xs ys s d1 d2.
+    OPTREL (λ(a,x) (b,y). a = b ∧ unthunk x y) d1 d2 ∧
     MAP FST xs = MAP FST ys ∧
     MAP (FST o SND) xs = MAP (FST o SND) ys ∧
     LIST_REL unthunk (MAP (SND o SND) xs) (MAP (SND o SND) ys) ⇒
-    unthunk (state_caseProof$rows_of s xs) (state_caseProof$rows_of s ys)
+    unthunk (state_caseProof$rows_of s xs d1) (state_caseProof$rows_of s ys d2)
 Proof
   Induct \\ Cases_on ‘ys’ \\ fs [state_caseProofTheory.rows_of_def]
-  >- (irule_at Any state_unthunkProofTheory.compile_rel_App \\ fs [])
+  >-
+   (rw []
+    \\ Cases_on ‘d1’ \\ Cases_on ‘d2’ \\ fs []
+    \\ rpt (irule_at Any state_unthunkProofTheory.compile_rel_App \\ fs [])
+    \\ PairCases_on ‘x’
+    \\ PairCases_on ‘x'’ \\ fs []
+    \\ rpt (irule_at Any state_unthunkProofTheory.compile_rel_If \\ fs [])
+    \\ rpt (irule_at Any state_unthunkProofTheory.compile_rel_App \\ fs [])
+    \\ fs [unthnk_Disj])
   \\ PairCases \\ PairCases_on ‘h’ \\ fs [] \\ rw []
   \\ fs [state_caseProofTheory.rows_of_def]
   \\ irule_at Any state_unthunkProofTheory.compile_rel_If \\ fs []
   \\ irule_at Any state_unthunkProofTheory.compile_rel_App \\ fs []
-  \\ irule_at Any state_unthunkProofTheory.compile_rel_Let \\ fs []
   \\ irule_at Any state_unthunkProofTheory.compile_rel_Var \\ fs []
   \\ irule unthunk_lets_for
   \\ fs []
@@ -127,37 +149,42 @@ QED
 Theorem to_state_lets_for:
   ∀xs v h1 h2.
     to_state h1 h2 ∧ v ∉ monad_cns ⇒
-    to_state (lets_for v s xs h1)
-             (state_caseProof$lets_for v s xs h2)
+    to_state (lets_for l v s xs h1)
+             (state_caseProof$lets_for l v s xs h2)
 Proof
   Induct
   \\ fs [state_caseProofTheory.lets_for_def,envLangTheory.lets_for_def]
   \\ PairCases
   \\ fs [state_caseProofTheory.lets_for_def,envLangTheory.lets_for_def] \\ rw []
   \\ irule_at Any env_to_state_1ProofTheory.compile_rel_Let \\ fs []
+  \\ irule_at Any env_to_state_1ProofTheory.compile_rel_Let \\ fs []
+  \\ irule_at Any env_to_state_1ProofTheory.compile_rel_If \\ fs []
   \\ irule_at Any env_to_state_1ProofTheory.compile_rel_Proj \\ fs []
   \\ irule_at Any env_to_state_1ProofTheory.compile_rel_Var \\ fs []
+  \\ irule_at Any env_to_state_1ProofTheory.compile_rel_Cons \\ fs []
+  \\ irule_at Any env_to_state_1ProofTheory.compile_rel_IsEq \\ fs []
+  \\ irule_at Any env_to_state_1ProofTheory.compile_rel_Var \\ fs []
+  \\ fs [EVAL “monad_cns”]
+  \\ cheat (* fail and fail *)
 QED
 
 Theorem to_state_rows_of:
-  ∀xs ys s.
+  ∀xs ys s d1 d2.
     MAP FST xs = MAP FST ys ∧
     MAP (FST o SND) xs = MAP (FST o SND) ys ∧
     DISJOINT (set (MAP FST xs)) monad_cns ∧
     LIST_REL to_state (MAP (SND o SND) xs) (MAP (SND o SND) ys) ⇒
-    to_state (rows_of s xs) (state_caseProof$rows_of s ys)
+    to_state (rows_of s xs d1) (state_caseProof$rows_of s ys d2)
 Proof
   Induct \\ Cases_on ‘ys’
   \\ fs [state_caseProofTheory.rows_of_def,
          envLangTheory.rows_of_def]
-  >- (irule_at Any env_to_state_1ProofTheory.compile_rel_AtomOp \\ fs [])
+  >- cheat (* (irule_at Any env_to_state_1ProofTheory.compile_rel_AtomOp \\ fs []) *)
   \\ PairCases \\ PairCases_on ‘h’ \\ fs [] \\ rw []
   \\ fs [state_caseProofTheory.rows_of_def,
          envLangTheory.rows_of_def]
   \\ irule_at Any env_to_state_1ProofTheory.compile_rel_If \\ fs []
   \\ irule_at Any env_to_state_1ProofTheory.compile_rel_IsEq \\ fs []
-  \\ irule_at Any env_to_state_1ProofTheory.compile_rel_Var \\ fs []
-  \\ irule_at Any env_to_state_1ProofTheory.compile_rel_Let \\ fs []
   \\ irule_at Any env_to_state_1ProofTheory.compile_rel_Var \\ fs []
   \\ irule to_state_lets_for \\ fs []
 QED
@@ -258,9 +285,11 @@ Proof
 QED
 
 Triviality expand_Case_neq:
-  state_caseProof$expand_Case se v ses ≠ Lam x t
+  state_caseProof$expand_Case v ses se ≠ Lam x t
 Proof
   rw [state_caseProofTheory.expand_Case_def]
+  \\ Cases_on ‘ses’ \\ fs [state_caseProofTheory.rows_of_def]
+  \\ PairCases_on ‘h’ \\ fs [state_caseProofTheory.rows_of_def]
 QED
 
 Theorem Letrec_split_names:
@@ -275,6 +304,7 @@ Theorem Letrec_split_names:
     MAP (FST ∘ SND) delays = MAP (FST ∘ SND) delays' ∧
     MAP (explode ∘ FST) funs = MAP FST funs'
 Proof
+  cheat (*
   Induct
   \\ fs [Letrec_split_def,state_unthunkProofTheory.Letrec_split_def,PULL_EXISTS]
   \\ PairCases \\ fs []
@@ -314,7 +344,7 @@ Proof
   \\ simp [Once env_to_state_1ProofTheory.compile_rel_cases]
   \\ strip_tac \\ gvs []
   \\ Cases_on ‘m’ \\ gvs []
-  \\ fs [Letrec_imm_def,state_unthunkProofTheory.Letrec_imm_def]
+  \\ fs [Letrec_imm_def,state_unthunkProofTheory.Letrec_imm_def] *)
 QED
 
 Theorem clean_Ref:
@@ -353,6 +383,7 @@ Theorem Letrec_split_case_clean:
       LIST_REL clean ds (MAP (to_state o SND o SND) delays) ∧
       LIST_REL clean fs (MAP (λ(f,n,x). Lam (SOME n) (to_state x)) funs)
 Proof
+  cheat (*
   Induct
   \\ fs [Letrec_split_def,state_unthunkProofTheory.Letrec_split_def,PULL_EXISTS]
   \\ PairCases \\ fs []
@@ -396,7 +427,7 @@ Proof
   \\ pop_assum $ irule_at Any
   \\ drule clean_Ref \\ fs []
   \\ rw []
-  \\ drule clean_Lam \\ fs []
+  \\ drule clean_Lam \\ fs [] *)
 QED
 
 Definition body_of_def[simp]:
@@ -807,6 +838,7 @@ Proof
     \\ rpt $ first_x_assum $ irule_at $ Pos hd
     \\ rpt (irule_at Any state_caseProofTheory.compile_rel_If \\ fs [PULL_EXISTS]))
   >~ [‘Case’] >-
+   cheat (*
    (rw [to_state_def] \\ fs [combined_def]
     \\ rpt (irule_at Any state_app_unitProofTheory.cexp_rel_Case \\ fs [PULL_EXISTS])
     \\ rpt $ first_x_assum $ irule_at $ Pos hd
@@ -862,7 +894,7 @@ Proof
     \\ fs [UNCURRY,MAP_MAP_o,combinTheory.o_DEF]
     \\ Induct
     \\ fs [PULL_EXISTS,PULL_FORALL]
-    \\ Cases_on ‘rs'’ \\ fs [] \\ metis_tac [])
+    \\ Cases_on ‘rs'’ \\ fs [] \\ metis_tac []) *)
   >~ [‘Letrec’] >-
    (rw [to_state_def] \\ fs [combined_def]
     \\ rpt $ irule_at Any env_to_state_1ProofTheory.compile_rel_Letrec
