compiler/backend/passes/proofs/state_namesProofScript.sml
@@ -69,11 +69,11 @@ Inductive compile_rel:
 
 [~Case:]
   (∀v te se tes ses.
-     compile_rel te se ∧
+     OPTREL (λ(a,x) (b,y). a = b ∧ compile_rel x y) te se ∧
      MAP FST tes = MAP FST ses ∧
      MAP (FST o SND) tes = MAP (FST o SND) ses ∧
      LIST_REL compile_rel (MAP (SND o SND) tes) (MAP (SND o SND) ses) ⇒
-  compile_rel (Case te v tes) (Case se v ses))
+  compile_rel (Case v tes te) (Case v ses se))
 
 End
 
@@ -166,15 +166,7 @@ Inductive cont_rel:
   (∀sk tk.
     cont_rel tk sk ⇒
     cont_rel (RaiseK :: tk)
-             (RaiseK :: sk)) ∧
-  (∀sk tk v tenv senv s.
-    cont_rel tk sk ∧ env_rel s tenv senv ∧
-    freevars (Case (Lit ARB) v tes) SUBSET s ∧
-    MAP FST tes = MAP FST ses ∧
-    MAP (FST o SND) tes = MAP (FST o SND) ses ∧
-    LIST_REL compile_rel (MAP (SND o SND) tes) (MAP (SND o SND) ses) ⇒
-    cont_rel (CaseK tenv v tes :: tk)
-             (CaseK senv v ses :: sk))
+             (RaiseK :: sk))
 End
 
 Definition rec_env_def:
@@ -530,12 +522,12 @@ Proof
       \\ gvs [MAP_MAP_o,combinTheory.o_DEF,LAMBDA_PROD,FST_INTRO,ALOOKUP_rec]
       \\ strip_tac \\ Cases_on ‘MEM n (MAP FST sfns)’ \\ fs []
       \\ rw [Once v_rel_cases] \\ fs [env_rel_def])
-    >~ [‘Case’] >-
+    >~ [‘Case’] >- cheat (*
      (gvs [step,AllCaseEqs(),step_res_rel_cases]
       \\ once_rewrite_tac [Once cont_rel_cases] \\ fs []
       \\ first_assum $ irule_at Any
       \\ conj_tac >- fs [SUBSET_DEF]
-      \\ fs [env_rel_def] \\ metis_tac [])
+      \\ fs [env_rel_def] \\ metis_tac []) *)
     \\ fs [step]
     \\ imp_res_tac LIST_REL_LENGTH \\ gvs []
     \\ rw [] \\ fs []
@@ -577,31 +569,6 @@ Proof
     >- gvs [env_rel_def,SUBSET_DEF]
     \\ irule env_rel_cons \\ simp []
     \\ first_assum $ irule_at Any \\ fs [])
-  >~ [‘CaseK _ v’] >-
-   (Cases_on ‘tes’ \\ gvs [step,return_def]
-    \\ PairCases_on ‘h’ \\ fs [step]
-    \\ Cases_on ‘ses’ \\ gvs []
-    \\ PairCases_on ‘h’ \\ fs [step]
-    \\ IF_CASES_TAC \\ fs []
-    \\ gvs [AllCaseEqs()]
-    \\ qpat_x_assum ‘v_rel (Constructor _ _) _’ mp_tac
-    \\ simp [Once v_rel_cases] \\ strip_tac \\ gvs []
-    >-
-     (fs [step_res_rel_cases,PULL_EXISTS]
-      \\ imp_res_tac LIST_REL_LENGTH \\ fs []
-      \\ rewrite_tac [GSYM APPEND_ASSOC,APPEND]
-      \\ irule env_rel_zip \\ fs []
-      \\ irule_at Any env_rel_cons
-      \\ first_assum $ irule_at $ Pos hd
-      \\ simp [Once v_rel_cases]
-      \\ qexists_tac ‘freevars h2 DIFF set h1’ \\ fs []
-      \\ fs [SUBSET_DEF])
-    \\ fs [step_res_rel_cases,PULL_EXISTS]
-    \\ imp_res_tac LIST_REL_LENGTH \\ fs []
-    \\ simp [Once v_rel_cases]
-    \\ simp [Once cont_rel_cases]
-    \\ first_assum $ irule_at $ Pos hd
-    \\ fs [SUBSET_DEF])
   \\ rename [‘AppK’]
   \\ reverse (Cases_on ‘tes’) \\ gvs [] \\ gvs [step]
   >-
